ProofLibrary/TermBasics.lean
@@ -1,5 +1,7 @@
 import ProofLibrary.List
 import ProofLibrary.FiniteTree
+import ProofLibrary.Set.Basic
+import ProofLibrary.Set.Finite
 
 structure Signature where
   P : Type u
@@ -38,6 +40,32 @@ def GroundTerm.toConst (t : GroundTerm sig) (isConst : ∃ c, t = GroundTerm.con
     apply False.elim
     rcases isConst with ⟨c, isConst⟩
     simp [GroundTerm.const] at isConst
+
+def GroundTerm.contains_func (func : SkolemFS sig) : GroundTerm sig -> Bool
+| .leaf _ => false
+| .inner func' ts => func == func' || ts.toList.attach.any (fun ⟨t, mem⟩ =>
+  have : t.depth < (FiniteTree.inner func' ts).depth := by
+    conv => right; unfold FiniteTree.depth
+    rw [Nat.add_comm]
+    apply Nat.lt_add_one_of_le
+    apply FiniteTree.depth_le_depthList_of_mem
+    exact mem
+  contains_func func t
+)
+termination_by t => FiniteTree.depth t
+
+def GroundTerm.cyclic : GroundTerm sig -> Bool
+| .leaf _ => false
+| .inner func ts => (ts.toList.any (contains_func func)) || ts.toList.attach.any (fun ⟨t, mem⟩ =>
+  have : t.depth < (FiniteTree.inner func ts).depth := by
+    conv => right; unfold FiniteTree.depth
+    rw [Nat.add_comm]
+    apply Nat.lt_add_one_of_le
+    apply FiniteTree.depth_le_depthList_of_mem
+    exact mem
+  cyclic t
+)
+termination_by t => FiniteTree.depth t
 
 def SkolemTerm.variables : SkolemTerm sig -> List sig.V
   | .var v => List.cons v List.nil
@@ -146,3 +174,60 @@ namespace VarOrConst
 
 end VarOrConst
 
+
+section ListsOfTerms
+
+  variable {sig : Signature} [DecidableEq sig.C] [DecidableEq sig.V]
+
+  def all_term_lists_of_length (candidate_terms : List (GroundTerm sig)) : Nat -> List (List (GroundTerm sig))
+  | .zero => [[]]
+  | .succ n =>
+    let prev_terms := all_term_lists_of_length candidate_terms n
+    candidate_terms.flatMap (fun t =>
+      prev_terms.map (fun ts =>
+        t :: ts
+      )
+    )
+
+  theorem mem_all_term_lists_of_length (candidate_terms : List (GroundTerm sig)) (length : Nat) : ∀ ts, ts ∈ (all_term_lists_of_length candidate_terms length) ↔ (ts.length = length ∧ (∀ t, t ∈ ts -> t ∈ candidate_terms)) := by
+    induction length with
+    | zero => intro ts; unfold all_term_lists_of_length; simp; intro eq t mem; rw [eq] at mem; simp at mem
+    | succ length ih =>
+      intro ts
+      unfold all_term_lists_of_length
+      simp only [List.mem_flatMap, List.mem_map]
+
+      constructor
+      . intro h
+        rcases h with ⟨t, t_mem, prev, prev_mem, ts_eq⟩
+        rw [← ts_eq]
+        specialize ih prev
+        have ih := ih.mp prev_mem
+        constructor
+        . rw [List.length_cons, ih.left]
+        . intro t' t'_mem
+          rw [List.mem_cons] at t'_mem
+          cases t'_mem with
+          | inl t'_mem => rw [t'_mem]; apply t_mem
+          | inr t'_mem => apply ih.right; exact t'_mem
+      . intro h
+        cases ts with
+        | nil => simp at h
+        | cons hd tl =>
+          exists hd
+          constructor
+          . apply h.right
+            simp
+          . exists tl
+            constructor
+            . rw [ih]
+              constructor
+              . have l := h.left
+                rw [List.length_cons, Nat.add_right_cancel_iff] at l
+                exact l
+              . intro t t_mem
+                apply h.right
+                simp [t_mem]
+            . rfl
+
+end ListsOfTerms
